Finish the adequacy regarding threads

simulations/simglobal/SimGlobal.v
@@ -14,231 +14,164 @@ Require Import SimSTS.
 
 Set Implicit Arguments.
 
-Section SIM.
+Definition smj : Type := option bool.
 
-Section TY.
-(* Context `{R: Type}. *)
-Inductive _simg
-          (simg: forall R0 R1 (RR: R0 -> R1 -> Prop), bool -> bool -> (itree coreE R0) -> (itree coreE R1) -> Prop)
-          {R0 R1} (RR: R0 -> R1 -> Prop) (f_src f_tgt: bool): (itree coreE R0) -> (itree coreE R1) -> Prop :=
-| simg_ret
-    r_src r_tgt
-    (SIM: RR r_src r_tgt)
-  :
-    _simg simg RR f_src f_tgt (Ret r_src) (Ret r_tgt)
-| simg_io
-    I O ktr_src0 ktr_tgt0 fn (varg: I)
-    (SIM: forall (x_src x_tgt: O) (EQ: x_src = x_tgt), simg _ _ RR true true (ktr_src0 x_src) (ktr_tgt0 x_tgt))
-  :
-    _simg simg RR f_src f_tgt (trigger (IO fn varg) >>= ktr_src0) (trigger (IO fn varg) >>= ktr_tgt0)
+Definition smj_top :smj := None.
+Definition smj_mid :smj := Some true.
+Definition smj_bot :smj := Some false.
 
-| simg_tauL
-    itr_src0 itr_tgt0
-    (TAUL: True)
-    (SIM: @_simg simg _ _ RR true f_tgt itr_src0 itr_tgt0)
-  :
-    _simg simg RR f_src f_tgt (tau;; itr_src0) (itr_tgt0)
-| simg_tauR
-    itr_src0 itr_tgt0
-    (TAUR: True)
-    (SIM: @_simg simg _ _ RR f_src true itr_src0 itr_tgt0)
-  :
-    _simg simg RR f_src f_tgt (itr_src0) (tau;; itr_tgt0)
+Definition smj_ltb (m1 m2: smj) : bool :=
+  match m1, m2 with
+  | Some _, None => true
+  | Some false, Some true => true
+  | _, _ => false
+  end.
 
-| simg_chooseL
-    X ktr_src0 itr_tgt0
-    (CHOOSEL: True)
-    (SIM: exists x, _simg simg RR true f_tgt (ktr_src0 x) itr_tgt0)
-  :
-    _simg simg RR f_src f_tgt (trigger (Choose X) >>= ktr_src0) (itr_tgt0)
-| simg_chooseR
-    X itr_src0 ktr_tgt0
-    (CHOOSER: True)
-    (SIM: forall x, _simg simg RR f_src true itr_src0 (ktr_tgt0 x))
-  :
-    _simg simg RR f_src f_tgt (itr_src0) (trigger (Choose X) >>= ktr_tgt0)
+Definition smj_leb m1 m2 :=
+  negb (smj_ltb m2 m1).
 
-| simg_takeL
-    X ktr_src0 itr_tgt0
-    (TAKEL: True)
-    (SIM: forall x, _simg simg RR true f_tgt (ktr_src0 x) itr_tgt0)
-  :
-    _simg simg RR f_src f_tgt (trigger (Take X) >>= ktr_src0) (itr_tgt0)
-| simg_takeR
-    X itr_src0 ktr_tgt0
-    (TAKER: True)
-    (SIM: exists x, _simg simg RR f_src true itr_src0 (ktr_tgt0 x))
-  :
-    _simg simg RR f_src f_tgt (itr_src0) (trigger (Take X) >>= ktr_tgt0)
+Definition smj_le m1 m2 :=
+  m1 = m2 \/ smj_ltb m1 m2.
 
-| simg_progress
-    itr_src itr_tgt
-    (SIM: simg _ _ RR false false itr_src itr_tgt)
-    (SRC: f_src = true)
-    (TGT: f_tgt = true)
-  :
-    _simg simg RR f_src f_tgt itr_src itr_tgt
-.
+Hint Unfold smj_le.
 
-Lemma _simg_ind2 (r: forall R0 R1 (RR: R0 -> R1 -> Prop), bool -> bool -> (itree coreE R0) -> (itree coreE R1) -> Prop)
-      R0 R1 (RR: R0 -> R1 -> Prop)
-      (P: bool -> bool -> (itree coreE R0) -> (itree coreE R1) -> Prop)
-      (RET: forall
-          f_src f_tgt
-          r_src r_tgt
-          (SIM: RR r_src r_tgt),
-          P f_src f_tgt (Ret r_src) (Ret r_tgt))
-      (IO: forall
-          f_src f_tgt
-          I O ktr_src0 ktr_tgt0 fn (varg: I)
-          (SIM: forall (x_src x_tgt:O) (EQ: x_src = x_tgt), r _ _ RR true true (ktr_src0 x_src) (ktr_tgt0 x_tgt)),
-          P f_src f_tgt (trigger (IO fn varg) >>= ktr_src0) (trigger (IO fn varg) >>= ktr_tgt0))
-      (TAUL: forall
-          f_src f_tgt
-          itr_src0 itr_tgt0
-          (TAUL: True)
-          (SIM: _simg r RR true f_tgt itr_src0 itr_tgt0)
-          (IH: P true f_tgt itr_src0 itr_tgt0),
-          P f_src f_tgt (tau;; itr_src0) (itr_tgt0))
-      (TAUR: forall
-          f_src f_tgt
-          itr_src0 itr_tgt0
-          (TAUR: True)
-          (SIM: _simg r RR f_src true itr_src0 itr_tgt0)
-          (IH: P f_src true itr_src0 itr_tgt0),
-          P f_src f_tgt (itr_src0) (tau;;itr_tgt0))
-      (CHOOSEL: forall
-          f_src f_tgt
-          X ktr_src0 itr_tgt0
-          (CHOOSEL: True)
-          (SIM: exists x, <<SIM: _simg r RR true f_tgt (ktr_src0 x) itr_tgt0>> /\ <<IH: P true f_tgt (ktr_src0 x) itr_tgt0>>),
-          P f_src f_tgt (trigger (Choose X) >>= ktr_src0) (itr_tgt0))
-      (CHOOSER: forall
-          f_src f_tgt
-          X itr_src0 ktr_tgt0
-          (CHOOSER: True)
-          (SIM: forall x, <<SIM: _simg r RR f_src true itr_src0 (ktr_tgt0 x)>> /\ <<IH: P f_src true itr_src0 (ktr_tgt0 x)>>),
-          P f_src f_tgt (itr_src0) (trigger (Choose X) >>= ktr_tgt0))
-      (TAKEL: forall
-          f_src f_tgt
-          X ktr_src0 itr_tgt0
-          (TAKEL: True)
-          (SIM: forall x, <<SIM: _simg r RR true f_tgt (ktr_src0 x) itr_tgt0>> /\ <<IH: P true f_tgt (ktr_src0 x) itr_tgt0>>),
-          P f_src f_tgt (trigger (Take X) >>= ktr_src0) (itr_tgt0))
-      (TAKER: forall
-          f_src f_tgt
-          X itr_src0 ktr_tgt0
-          (TAKER: True)
-          (SIM: exists x, <<SIM: _simg r RR f_src true itr_src0 (ktr_tgt0 x)>> /\ <<IH: P f_src true itr_src0 (ktr_tgt0 x)>>),
-          P f_src f_tgt (itr_src0) (trigger (Take X) >>= ktr_tgt0))
-      (PROGRESS: forall
-          f_src f_tgt
-          itr_src itr_tgt
-          (SIM: r _ _ RR false false itr_src itr_tgt)
-          (SRC: f_src = true)
-          (TGT: f_tgt = true),
-          P f_src f_tgt itr_src itr_tgt)
+Lemma smj_ltb_trans m1 m2 m3
+  (LT1: smj_ltb m1 m2)
+  (LT2: smj_ltb m2 m3)
   :
-    forall f_src f_tgt itr_src itr_tgt
-           (SIM: _simg r RR f_src f_tgt itr_src itr_tgt),
-      P f_src f_tgt itr_src itr_tgt.
+  smj_ltb m1 m3.
+Proof. destruct m1, m2, m3; ss; des_ifs. Qed.
+
+Lemma smj_lt_mid_top:
+  smj_ltb smj_mid smj_top.
+Proof. ss. Qed.
+
+Lemma smj_le_bot m:
+  smj_le smj_bot m.
 Proof.
-  fix IH 5. i. inv SIM.
-  { eapply RET; eauto. }
-  { eapply IO; eauto. }
-  { eapply TAUL; eauto. }
-  { eapply TAUR; eauto. }
-  { eapply CHOOSEL; eauto. des. esplits; eauto. }
-  { eapply CHOOSER; eauto. }
-  { eapply TAKEL; eauto. }
-  { eapply TAKER; eauto. des. esplits; eauto. }
-  { eapply PROGRESS; eauto. }
+  destruct m as [[] | ]; ss; eauto.
 Qed.
 
-Definition simg: forall R0 R1 (RR: R0 -> R1 -> Prop), bool -> bool -> (itree coreE R0) -> (itree coreE R1) -> Prop := paco7 _simg bot7.
+Variant simg_def
+  (simg: forall R0 R1 (RR: R0 -> R1 -> Prop), smj -> smj -> (itree coreE R0) -> (itree coreE R1) -> Prop)
+  {R0 R1} (RR: R0 -> R1 -> Prop)           
+  (self:  smj -> smj -> (itree coreE R0) -> (itree coreE R1) -> Prop):
+  smj -> smj -> (itree coreE R0) -> (itree coreE R1) -> Prop :=
+
+| simg_ret ps pt
+  r_src r_tgt
+  (SIM: RR r_src r_tgt)
+:
+simg_def simg RR self ps pt (Ret r_src) (Ret r_tgt)
+
+| simg_io ps pt ps0 pt0
+  I O ktr_src0 ktr_tgt0 fn (varg: I)
+  (SIM: forall (x_src x_tgt: O) (EQ: x_src = x_tgt), self ps0 pt0 (ktr_src0 x_src) (ktr_tgt0 x_tgt))
+:
+simg_def simg RR self ps pt (trigger (IO fn varg) >>= ktr_src0) (trigger (IO fn varg) >>= ktr_tgt0)
+
+| simg_tauL ps pt ps0
+  itr_src0 itr_tgt0
+  (SIM: self ps0 pt itr_src0 itr_tgt0)
+:
+simg_def simg RR self ps pt (tau;; itr_src0) (itr_tgt0)
+
+| simg_tauR ps pt pt0
+  itr_src0 itr_tgt0
+  (SIM: self ps pt0 itr_src0 itr_tgt0)
+:
+simg_def simg RR self ps pt (itr_src0) (tau;; itr_tgt0)
+
+| simg_chooseL ps pt ps0
+  X ktr_src0 itr_tgt0
+  (SIM: exists x, self ps0 pt (ktr_src0 x) itr_tgt0)
+:
+simg_def simg RR self ps pt (trigger (Choose X) >>= ktr_src0) (itr_tgt0)
+
+| simg_chooseR ps pt pt0
+  X itr_src0 ktr_tgt0
+  (SIM: forall x, self ps pt0 itr_src0 (ktr_tgt0 x))
+:
+simg_def simg RR self ps pt (itr_src0) (trigger (Choose X) >>= ktr_tgt0)
+
+| simg_takeL ps pt ps0
+  X ktr_src0 itr_tgt0
+  (SIM: forall x, self ps0 pt (ktr_src0 x) itr_tgt0)
+:
+  simg_def simg RR self ps pt (trigger (Take X) >>= ktr_src0) (itr_tgt0)
+
+| simg_takeR ps pt pt0
+  X itr_src0 ktr_tgt0
+  (SIM: exists x, self ps pt0 itr_src0 (ktr_tgt0 x))
+:
+  simg_def simg RR self ps pt (itr_src0) (trigger (Take X) >>= ktr_tgt0)
+
+| simg_progress ps pt ps0 pt0
+  itr_src itr_tgt
+  (SIM: simg _ _ RR ps0 pt0 itr_src itr_tgt)
+  (DECS: smj_ltb ps0 ps)
+  (DECT: smj_ltb pt0 pt)
+:
+simg_def simg RR self ps pt itr_src itr_tgt
+.
+
+Lemma simg_def_mon simg simg' R_src R_tgt RR P P'
+  (LESIM: simg <7= simg')
+  (LE: P <4= P')
+  :
+  @simg_def simg R_src R_tgt RR P <4= simg_def simg' RR P'.
+Proof.
+  i. destruct PR; des; eauto using simg_def.
+Qed.
+
+Inductive _simg simg {R0 R1} RR ps pt isrc itgt : Prop :=
+| _simg_intro (SIM: @simg_def simg R0 R1 RR (_simg simg RR) ps pt isrc itgt)
+.
+
+Lemma simg_tarski (simg: forall R0 R1 (RR: R0 -> R1 -> Prop), smj -> smj -> (itree coreE R0) -> (itree coreE R1) -> Prop)
+    R0 R1 (RR: R0 -> R1 -> Prop)
+    (P: smj -> smj -> (itree coreE R0) -> (itree coreE R1) -> Prop)
+  (SIM: simg_def simg RR P <4= P)
+  :
+  _simg simg RR <4= P.
+Proof.
+  fix IH 5. i. inv PR; inv SIM0; eapply SIM; des; econs; try eapply IH; eauto.
+Qed.
+
+Definition simg: forall R0 R1 (RR: R0 -> R1 -> Prop),  smj -> smj -> (itree coreE R0) -> (itree coreE R1) -> Prop :=
+  paco7 _simg bot7.
 
 Lemma simg_mon: monotone7 _simg.
 Proof.
-  ii. induction IN using _simg_ind2.
-  { econs 1; eauto. }
-  { econs 2; eauto. }
-  { econs 3; eauto. }
-  { econs 4; eauto. }
-  { econs 5; eauto. des. esplits; eauto. }
-  { econs 6; eauto. i. exploit SIM; eauto. des. i. des. eauto. }
-  { econs 7; eauto. i. exploit SIM; eauto. des. i. des. eauto. }
-  { econs 8; eauto. des. esplits; eauto. }
-  { econs 9; eauto. }
+  ii. eapply simg_tarski, IN. i. inv PR; eauto using _simg, simg_def.
 Qed.
 Hint Resolve simg_mon: paco.
 Hint Resolve cpn7_wcompat: paco.
 
+Lemma simg_ind
+    R0 R1 (RR: R0 -> R1 -> Prop)
+    (P: smj -> smj -> (itree coreE R0) -> (itree coreE R1) -> Prop)
+  (SIM: simg_def simg RR (simg RR /4\ P) <4= P)
+  :
+  simg RR <4= P.
+Proof.
+  i. punfold PR.
+  assert (SIM': simg_def simg RR (simg RR /4\ P) <4= (simg RR /4\ P)).
+  { i. split; eauto. pstep. econs.
+    eapply simg_def_mon, PR0; eauto.
+    i. ss. des. punfold PR1. }
 
-Inductive simg_indC
-          (simg: forall R0 R1 (RR: R0 -> R1 -> Prop), bool -> bool -> (itree coreE R0) -> (itree coreE R1) -> Prop)
-          {R0 R1} (RR: R0 -> R1 -> Prop) (f_src f_tgt: bool): (itree coreE R0) -> (itree coreE R1) -> Prop :=
-| simg_indC_ret
-    r_src r_tgt
-    (SIM: RR r_src r_tgt)
-  :
-    simg_indC simg RR f_src f_tgt (Ret r_src) (Ret r_tgt)
-| simg_indC_syscall
-    I O ktr_src0 ktr_tgt0 fn (varg: I)
-    (SIM: forall (x_src x_tgt: O) (EQ: x_src = x_tgt), simg _ _ RR true true (ktr_src0 x_src) (ktr_tgt0 x_tgt))
-  :
-    simg_indC simg RR f_src f_tgt (trigger (IO fn varg) >>= ktr_src0) (trigger (IO fn varg) >>= ktr_tgt0)
+  eapply simg_tarski in SIM'; des; eauto.
+  eapply simg_mon; eauto. i. pclearbot. eauto.
+Qed.
 
-| simg_indC_tauL
-    itr_src0 itr_tgt0
-    (TAUL: True)
-    (SIM: simg _ _ RR true f_tgt itr_src0 itr_tgt0)
-  :
-    simg_indC simg RR f_src f_tgt (tau;; itr_src0) (itr_tgt0)
-| simg_indC_tauR
-    itr_src0 itr_tgt0
-    (TAUR: True)
-    (SIM: simg _ _ RR f_src true itr_src0 itr_tgt0)
-  :
-    simg_indC simg RR f_src f_tgt (itr_src0) (tau;; itr_tgt0)
-
-| simg_indC_chooseL
-    X ktr_src0 itr_tgt0
-    (CHOOSEL: True)
-    (SIM: exists x, simg _ _ RR true f_tgt (ktr_src0 x) itr_tgt0)
-  :
-    simg_indC simg RR f_src f_tgt (trigger (Choose X) >>= ktr_src0) (itr_tgt0)
-| simg_indC_chooseR
-    X itr_src0 ktr_tgt0
-    (CHOOSER: True)
-    (SIM: forall x, simg _ _ RR f_src true itr_src0 (ktr_tgt0 x))
-  :
-    simg_indC simg RR f_src f_tgt (itr_src0) (trigger (Choose X) >>= ktr_tgt0)
-
-| simg_indC_takeL
-    X ktr_src0 itr_tgt0
-    (TAKEL: True)
-    (SIM: forall x, simg _ _ RR true f_tgt (ktr_src0 x) itr_tgt0)
-  :
-    simg_indC simg RR f_src f_tgt (trigger (Take X) >>= ktr_src0) (itr_tgt0)
-| simg_indC_takeR
-    X itr_src0 ktr_tgt0
-    (TAKER: True)
-    (SIM: exists x, simg _ _ RR f_src true itr_src0 (ktr_tgt0 x))
-  :
-    simg_indC simg RR f_src f_tgt (itr_src0) (trigger (Take X) >>= ktr_tgt0)
-.
+Definition simg_indC simg {R0 R1} RR :=
+  @simg_def bot7 R0 R1 RR (simg R0 R1 RR).
 
 Lemma simg_indC_mon: monotone7 simg_indC.
 Proof.
-  ii. inv IN.
-  { econs 1; eauto. }
-  { econs 2; eauto. }
-  { econs 3; eauto. }
-  { econs 4; eauto. }
-  { econs 5; eauto. des. esplits; eauto. }
-  { econs 6; eauto. }
-  { econs 7; eauto. }
-  { econs 8; eauto. des. esplits; eauto. }
+  ii. unfold simg_indC in *.
+  inv IN; des; eauto using simg_def.
 Qed.
 Hint Resolve simg_indC_mon: paco.
 
@@ -246,115 +179,30 @@ Lemma simg_indC_spec:
   simg_indC <8= gupaco7 _simg (cpn7 _simg).
 Proof.
   eapply wrespect7_uclo; eauto with paco.
-  econs; eauto with paco. i. inv PR.
-  { econs 1; eauto. }
-  { econs 2; eauto. i. eapply rclo7_base. auto. }
-  { econs 3; eauto. eapply simg_mon; eauto. i. eapply rclo7_base. auto. }
-  { econs 4; eauto. eapply simg_mon; eauto. i. eapply rclo7_base. auto. }
-  { des. econs 5; eauto. esplits. eapply simg_mon; eauto. i. eapply rclo7_base; eauto. }
-  { econs 6; eauto. i. eapply simg_mon; eauto. i. eapply rclo7_base; eauto. }
-  { econs 7; eauto. i. eapply simg_mon; eauto. i. eapply rclo7_base; eauto. }
-  { des. econs 8; eauto. esplits. eapply simg_mon; eauto. i. eapply rclo7_base; eauto. }
+  econs; eauto with paco. i.
+  inv PR; econs; des; subst; ss; eauto 7 using simg_def, simg_mon, rclo7.
 Qed.
-
-Lemma simg_ind R0 R1 (RR: R0 -> R1 -> Prop)
-      (P: bool -> bool -> (itree coreE R0) -> (itree coreE R1) -> Prop)
-      (RET: forall
-          f_src f_tgt
-          r_src r_tgt
-          (SIM: RR r_src r_tgt),
-          P f_src f_tgt (Ret r_src) (Ret r_tgt))
-      (IO: forall
-          f_src f_tgt
-          I O ktr_src0 ktr_tgt0 fn (varg: I)
-          (SIM: forall (x_src x_tgt: O) (EQ: x_src = x_tgt), simg RR true true (ktr_src0 x_src) (ktr_tgt0 x_tgt)),
-          P f_src f_tgt (trigger (IO fn varg) >>= ktr_src0) (trigger (IO fn varg) >>= ktr_tgt0))
-      (TAUL: forall
-          f_src f_tgt
-          itr_src0 itr_tgt0
-          (TAUL: True)
-          (SIM: simg RR true f_tgt itr_src0 itr_tgt0)
-          (IH: P true f_tgt itr_src0 itr_tgt0),
-          P f_src f_tgt (tau;; itr_src0) (itr_tgt0))
-      (TAUR: forall
-          f_src f_tgt
-          itr_src0 itr_tgt0
-          (TAUR: True)
-          (SIM: simg RR f_src true itr_src0 itr_tgt0)
-          (IH: P f_src true itr_src0 itr_tgt0),
-          P f_src f_tgt (itr_src0) (tau;;itr_tgt0))
-      (CHOOSEL: forall
-          f_src f_tgt
-          X ktr_src0 itr_tgt0
-          (CHOOSEL: True)
-          (SIM: exists x, <<SIM: simg RR true f_tgt (ktr_src0 x) itr_tgt0>> /\ <<IH: P true f_tgt (ktr_src0 x) itr_tgt0>>),
-          P f_src f_tgt (trigger (Choose X) >>= ktr_src0) (itr_tgt0))
-      (CHOOSER: forall
-          f_src f_tgt
-          X itr_src0 ktr_tgt0
-          (CHOOSER: True)
-          (SIM: forall x, <<SIM: simg RR f_src true itr_src0 (ktr_tgt0 x)>> /\ <<IH: P f_src true itr_src0 (ktr_tgt0 x)>>),
-          P f_src f_tgt (itr_src0) (trigger (Choose X) >>= ktr_tgt0))
-      (TAKEL: forall
-          f_src f_tgt
-          X ktr_src0 itr_tgt0
-          (TAKEL: True)
-          (SIM: forall x, <<SIM: simg RR true f_tgt (ktr_src0 x) itr_tgt0>> /\ <<IH: P true f_tgt (ktr_src0 x) itr_tgt0>>),
-          P f_src f_tgt (trigger (Take X) >>= ktr_src0) (itr_tgt0))
-      (TAKER: forall
-          f_src f_tgt
-          X itr_src0 ktr_tgt0
-          (TAKER: True)
-          (SIM: exists x, <<SIM: simg RR f_src true itr_src0 (ktr_tgt0 x)>> /\ <<IH: P f_src true itr_src0 (ktr_tgt0 x)>>),
-          P f_src f_tgt (itr_src0) (trigger (Take X) >>= ktr_tgt0))
-      (PROGRESS: forall
-          f_src f_tgt
-          itr_src itr_tgt
-          (SIM: simg RR false false itr_src itr_tgt)
-          (SRC: f_src = true)
-          (TGT: f_tgt = true),
-          P f_src f_tgt itr_src itr_tgt)
-  :
-    forall f_src f_tgt itr_src itr_tgt
-           (SIM: simg RR f_src f_tgt itr_src itr_tgt),
-      P f_src f_tgt itr_src itr_tgt.
-Proof.
-  i. punfold SIM. induction SIM using _simg_ind2; i; clarify.
-  { eapply RET; eauto. }
-  { eapply IO; eauto. i. exploit SIM; eauto. i. des. pclearbot. eauto. }
-  { eapply TAUL; eauto. pfold. auto. }
-  { eapply TAUR; eauto. pfold. auto. }
-  { eapply CHOOSEL; eauto. des. esplits; eauto. pfold. auto. }
-  { eapply CHOOSER; eauto. i. exploit SIM; eauto. i. des. esplits; eauto. pfold. auto. }
-  { eapply TAKEL; eauto. i. exploit SIM; eauto. i. des. esplits; eauto. pfold. auto. }
-  { eapply TAKER; eauto. des. esplits; eauto. pfold. auto. }
-  { eapply PROGRESS; eauto. pclearbot. auto. }
-Qed.
-
-End TY.
 
 Hint Constructors _simg.
 Hint Unfold simg.
-Hint Resolve simg_mon: paco.
-Hint Resolve cpn7_wcompat: paco.
 
-Variant flagC (r: forall S0 S1 (SS: S0 -> S1 -> Prop), bool -> bool -> (itree coreE S0) -> (itree coreE S1) -> Prop):
-  forall S0 S1 (SS: S0 -> S1 -> Prop), bool -> bool -> (itree coreE S0) -> (itree coreE S1) -> Prop :=
-| flagC_intro
-    f_src0 f_src1 f_tgt0 f_tgt1 R0 R1 (RR: R0 -> R1 -> Prop) itr_src itr_tgt
-    (SRC: f_src0 = true -> f_src1 = true)
-    (TGT: f_tgt0 = true -> f_tgt1 = true)
-    (SIM: r _ _ RR f_src0 f_tgt0 itr_src itr_tgt)
-  :
-    flagC r RR f_src1 f_tgt1 itr_src itr_tgt
+Variant flagC (r: forall S0 S1 (SS: S0 -> S1 -> Prop),  smj -> smj -> (itree coreE S0) -> (itree coreE S1) -> Prop):
+  forall S0 S1 (SS: S0 -> S1 -> Prop),  smj -> smj -> (itree coreE S0) -> (itree coreE S1) -> Prop :=
+  | flagC_intro
+      ps0 ps1 pt0 pt1 R0 R1 (RR: R0 -> R1 -> Prop) itr_src itr_tgt
+      (SRC: smj_le ps0 ps1)
+      (TGT: smj_le pt0 pt1)
+      (SIM: r _ _ RR ps0 pt0 itr_src itr_tgt)
+    :
+    flagC r RR ps1 pt1 itr_src itr_tgt
 .
 Hint Constructors flagC: core.
 
 Lemma flagC_mon
-      r1 r2
-      (LE: r1 <7= r2)
+  r1 r2
+  (LE: r1 <7= r2)
   :
-    flagC r1 <7= flagC r2
+  flagC r1 <7= flagC r2
 .
 Proof. ii. destruct PR; econs; et. Qed.
 Hint Resolve flagC_mon: paco.
@@ -364,16 +212,12 @@ Proof.
   econs; eauto with paco.
   ii. inv PR. csc.
   eapply GF in SIM.
-  revert x3 x4 SRC TGT. induction SIM using _simg_ind2; i; clarify.
-  { econs 1; eauto. }
-  { econs 2; eauto. i. eapply rclo7_base; eauto. }
-  { econs 3; eauto. }
-  { econs 4; eauto. }
-  { econs 5; eauto. des. esplits; eauto. }
-  { econs 6; eauto. i. exploit SIM; eauto. i. des. eauto. }
-  { econs 7; eauto. i. exploit SIM; eauto. i. des. eauto. }
-  { econs 8; eauto. des. esplits; eauto. }
-  { econs 9; eauto. eapply rclo7_clo_base. econs; eauto. }
+  move SIM before GF. revert_until SIM.
+  pattern ps0, pt0, x5, x6.
+  eapply simg_tarski, SIM. i.
+  inv PR; des; econs; econs; i; subst; ss; eauto 7 using rclo7.
+  - destruct SRC; subst; eauto using smj_ltb_trans.
+  - destruct TGT; subst; eauto using smj_ltb_trans.
 Qed.
 
 Lemma flagC_spec: flagC <8= gupaco7 (_simg) (cpn7 (_simg)).
@@ -382,145 +226,67 @@ Proof.
 Qed.
 
 Lemma simg_flag
-      r R0 R1 RR itr_src itr_tgt f_src0 f_tgt0 f_src1 f_tgt1
-      (SIM: @_simg r R0 R1 RR f_src0 f_tgt0 itr_src itr_tgt)
-      (SRC: f_src0 = true -> f_src1 = true)
-      (TGT: f_tgt0 = true -> f_tgt1 = true)
+  r R0 R1 RR itr_src itr_tgt ps0 pt0 ps1 pt1
+  (SIM: @_simg r R0 R1 RR ps0 pt0 itr_src itr_tgt)
+  (SRC: smj_le ps0 ps1)
+  (TGT: smj_le pt0 pt1)
   :
-    @_simg r R0 R1 RR f_src1 f_tgt1 itr_src itr_tgt.
+  @_simg r R0 R1 RR ps1 pt1 itr_src itr_tgt.
 Proof.
-  revert f_src1 f_tgt1 SRC TGT. induction SIM using _simg_ind2; i.
-  { econs 1; eauto. }
-  { econs 2; eauto. }
-  { econs 3; eauto. }
-  { econs 4; eauto. }
-  { econs 5; eauto. des. esplits; eauto. }
-  { econs 6; eauto. i. exploit SIM; eauto. i. des. eauto. }
-  { econs 7; eauto. i. exploit SIM; eauto. i. des. eauto. }
-  { econs 8; eauto. des. esplits; eauto. }
-  { econs 9; eauto. }
+  move SIM before r. revert_until SIM.
+  pattern ps0, pt0, itr_src, itr_tgt.
+  eapply simg_tarski, SIM. i.
+  inv PR; des; econs; econs; i; subst; ss; eauto 7 using rclo7.
+  - destruct SRC; subst; eauto using smj_ltb_trans.
+  - destruct TGT; subst; eauto using smj_ltb_trans.
 Qed.
 
-Lemma simg_progress_flag R0 R1 RR r g itr_src itr_tgt
-      (SIM: gpaco7 _simg (cpn7 _simg) g g R0 R1 RR false false itr_src itr_tgt)
-  :
-    gpaco7 _simg (cpn7 _simg) r g R0 R1 RR true true itr_src itr_tgt.
-Proof.
-  gstep. econs; eauto.
-Qed.
+Variant bindR (r s: forall S0 S1 (SS: S0 -> S1 -> Prop),  smj -> smj -> (itree coreE S0) -> (itree coreE S1) -> Prop):
+  forall S0 S1 (SS: S0 -> S1 -> Prop), smj -> smj -> (itree coreE S0) -> (itree coreE S1) -> Prop :=
+  | bindR_intro ps pt
+      R0 R1 RR
+      (i_src: itree coreE R0) (i_tgt: itree coreE R1)
+      (SIM: r _ _ RR ps pt i_src i_tgt)
 
-Lemma simg_flag_down R0 R1 RR r g itr_src itr_tgt f_src f_tgt
-      (SIM: gpaco7 _simg (cpn7 _simg) r g R0 R1 RR false false itr_src itr_tgt)
-  :
-    gpaco7 _simg (cpn7 _simg) r g R0 R1 RR f_src f_tgt itr_src itr_tgt.
-Proof.
-  guclo flagC_spec. econs; [..|eauto]; ss.
-Qed.
-
-Lemma simg_bot_flag_up R0 R1 RR st_src st_tgt f_src f_tgt
-      (SIM: @simg R0 R1 RR true true st_src st_tgt)
-  :
-    simg RR f_src f_tgt st_src st_tgt.
-Proof.
-  ginit. remember true in SIM at 1. remember true in SIM at 1.
-  clear Heqb Heqb0. revert st_src st_tgt f_src f_tgt b b0 SIM.
-  gcofix CIH. i. revert f_src f_tgt.
-  induction SIM using simg_ind.
-  { guclo simg_indC_spec. econs 1; eauto. }
-  { gstep. econs 2; eauto. i. gbase. eapply CIH; eauto. }
-  { guclo simg_indC_spec. econs 3; eauto. }
-  { guclo simg_indC_spec. econs 4; eauto. }
-  { guclo simg_indC_spec. econs 5; eauto. des. esplits; eauto. }
-  { guclo simg_indC_spec. econs 6; eauto. i. hexploit SIM; eauto. i. des. esplits; eauto. }
-  { guclo simg_indC_spec. econs 7; eauto. i. hexploit SIM; eauto. i. des. esplits; eauto. }
-  { guclo simg_indC_spec. econs 8; eauto. des. esplits; eauto. }
-  { i. eapply simg_flag_down. gfinal. right.
-    eapply paco7_mon; eauto. ss.
-  }
-Qed.
-
-
-Variant bindR (r s: forall S0 S1 (SS: S0 -> S1 -> Prop), bool -> bool -> (itree coreE S0) -> (itree coreE S1) -> Prop):
-  forall S0 S1 (SS: S0 -> S1 -> Prop), bool -> bool -> (itree coreE S0) -> (itree coreE S1) -> Prop :=
-| bindR_intro
-    f_src f_tgt
-
-    R0 R1 RR
-    (i_src: itree coreE R0) (i_tgt: itree coreE R1)
-    (SIM: r _ _ RR f_src f_tgt i_src i_tgt)
-
-    S0 S1 SS
-    (k_src: ktree coreE R0 S0) (k_tgt: ktree coreE R1 S1)
-    (SIMK: forall vret_src vret_tgt (SIM: RR vret_src vret_tgt), s _ _ SS false false (k_src vret_src) (k_tgt vret_tgt))
-  :
-    bindR r s SS f_src f_tgt (ITree.bind i_src k_src) (ITree.bind i_tgt k_tgt)
+      S0 S1 SS
+      (k_src: ktree coreE R0 S0) (k_tgt: ktree coreE R1 S1)
+      (SIMK: forall vret_src vret_tgt (SIM: RR vret_src vret_tgt), s _ _ SS smj_bot smj_bot (k_src vret_src) (k_tgt vret_tgt))
+    :
+    bindR r s SS ps pt (ITree.bind i_src k_src) (ITree.bind i_tgt k_tgt)
 .
 
 Hint Constructors bindR: core.
 
 Lemma bindR_mon
-      r1 r2 s1 s2
-      (LEr: r1 <7= r2) (LEs: s1 <7= s2)
+  r1 r2 s1 s2
+  (LEr: r1 <7= r2) (LEs: s1 <7= s2)
   :
-    bindR r1 s1 <7= bindR r2 s2
+  bindR r1 s1 <7= bindR r2 s2
 .
 Proof. ii. destruct PR; econs; et. Qed.
 
 Definition bindC r := bindR r r.
 Hint Unfold bindC: core.
 
-
-
 Lemma bindC_wrespectful: wrespectful7 (_simg) bindC.
 Proof.
   econs.
   { ii. eapply bindR_mon; eauto. }
   i. inv PR. csc. eapply GF in SIM.
-  revert k_src k_tgt SIMK. induction SIM using _simg_ind2; i.
-  { irw. hexploit SIMK; eauto. i. eapply GF in H.
-    eapply simg_mon; eauto. eapply simg_flag.
-     { eapply simg_mon; eauto. i. eapply rclo7_base. auto. }
-    { ss. }
-    { ss. }
-  }
-  { rewrite ! bind_bind. econs; eauto. ii.
-    { econs 2; eauto with paco. econs; eauto with paco. }
-  }
-  { rewrite ! bind_tau. econs; eauto. }
-  { rewrite ! bind_tau. econs; eauto. }
-  { rewrite ! bind_bind. econs; eauto. des. esplits; et. }
-  { rewrite ! bind_bind. econs; eauto. i. exploit SIM; eauto. i. des. eauto. }
-  { rewrite ! bind_bind. econs; eauto. i. exploit SIM; eauto. i. des. eauto. }
-  { rewrite ! bind_bind. econs; eauto. des. esplits; et. }
-  { clarify. econs; eauto. eapply rclo7_clo_base. econs; eauto. }
+  move SIM before GF. revert_until SIM.
+  pattern x3, x4, i_src, i_tgt.
+  eapply simg_tarski, SIM. i.
+  inv PR; des; i; subst; ss; grind;
+    eauto 7 using simg_mon, simg_flag, simg_def, rclo7, smj_le_bot.
+
+  econs. econs; eauto.
+  econs 2; eauto 7 using simg_mon, simg_flag, simg_def, rclo7, smj_le_bot.
 Qed.
 
 Lemma bindC_spec: bindC <8= gupaco7 (_simg) (cpn7 (_simg)).
 Proof.
   intros. eapply wrespect7_uclo; eauto with paco. eapply bindC_wrespectful.
 Qed.
-
-Lemma self_simg:
-  forall (wf: Any.t -> Any.t -> Prop) (WF: forall x, wf x x) (itr: itree coreE Any.t), simg wf false false itr itr.
-Proof.
-  ginit. gcofix CIH. i. ides itr.
-  { gstep. econs; eauto. }
-  { gstep. econs; eauto. econs; eauto. econs; eauto. gbase. eauto. }
-  destruct e; rewrite <- bind_trigger; resub.
-  { 
-    gstep. econs 6; eauto. i. econs 5; eauto. exists x. 
-    econs; eauto. gbase. eauto.
-  }
-  {
-    gstep. econs; eauto. i. econs; eauto. exists x.
-    econs; eauto. gbase. eauto. 
-  }
-  {
-    gstep. econs; eauto. i. subst.
-    eapply simg_flag_down. gbase. eauto.  
-  }
-Qed.
-End SIM.
 
 Hint Constructors _simg.
 Hint Unfold simg.
@@ -529,95 +295,6 @@ Hint Constructors flagC: core.
 Hint Resolve flagC_mon: paco.
 Hint Constructors bindR: core.
 Hint Unfold bindC: core.
-Hint Constructors simg_indC: core.
+Hint Unfold simg_indC: core.
 Hint Resolve sim_indC_mon: paco.
 Hint Resolve cpn7_wcompat: paco.
-
-Variant _simg_safe
-          (simg: forall R0 R1 (RR: R0 -> R1 -> Prop), bool -> bool -> (itree coreE R0) -> (itree coreE R1) -> Prop)
-          {R0 R1} (RR: R0 -> R1 -> Prop) (f_src f_tgt: bool): (itree coreE R0) -> (itree coreE R1) -> Prop :=
-| simg_safe_ret
-    r_src r_tgt
-    (SIM: RR r_src r_tgt)
-  :
-    _simg_safe simg RR f_src f_tgt (Ret r_src) (Ret r_tgt)
-| simg_safe_syscall
-    I O ktr_src0 ktr_tgt0 fn (varg: I)
-    (SIM: forall (x_src x_tgt: O) (EQ: x_src = x_tgt), simg _ _ RR true true (ktr_src0 x_src) (ktr_tgt0 x_tgt))
-  :
-    _simg_safe simg RR f_src f_tgt (trigger (IO fn varg) >>= ktr_src0) (trigger (IO fn varg) >>= ktr_tgt0)
-
-| simg_safe_tauL
-    itr_src0 itr_tgt0
-    (TAUL: True)
-    (SIM: simg _ _ RR true f_tgt itr_src0 itr_tgt0)
-  :
-    _simg_safe simg RR f_src f_tgt (tau;; itr_src0) (itr_tgt0)
-| simg_safe_tauR
-    itr_src0 itr_tgt0
-    (TAUR: True)
-    (SIM: simg _ _ RR f_src true itr_src0 itr_tgt0)
-  :
-    _simg_safe simg RR f_src f_tgt (itr_src0) (tau;; itr_tgt0)
-
-| simg_safe_chooseR
-    X itr_src0 ktr_tgt0
-    (CHOOSER: True)
-    (SIM: forall x, simg _ _ RR f_src true itr_src0 (ktr_tgt0 x))
-  :
-    _simg_safe simg RR f_src f_tgt (itr_src0) (trigger (Choose X) >>= ktr_tgt0)
-
-| simg_safe_takeL
-    X ktr_src0 itr_tgt0
-    (TAKEL: True)
-    (SIM: forall x, simg _ _ RR true f_tgt (ktr_src0 x) itr_tgt0)
-  :
-    _simg_safe simg RR f_src f_tgt (trigger (Take X) >>= ktr_src0) (itr_tgt0)
-.
-
-Lemma simg_safe_spec:
-  _simg_safe <8= gupaco7 _simg (cpn7 _simg).
-Proof.
-  i. eapply simg_indC_spec. inv PR.
-  { econs; eauto. }
-  { econs; eauto. }
-  { econs; eauto. }
-  { econs; eauto. }
-  { econs; eauto. }
-  { econs; eauto. }
-Qed.
-
-(* Lemma simg_map R0 R1 RR R0' R1' RR' f_src f_tgt itl itr (f0: R0 -> R0') (f1: R1 -> R1')
-      (SIM: @simg R0 R1 RR f_src f_tgt itl itr)
-      (IMPL: forall r0 r1, RR r0 r1 -> RR' (f0 r0) (f1 r1): Prop)
-:
-      @simg R0' R1' RR' f_src f_tgt (f0 <$> itl) (f1 <$> itr)
-.
-Proof.
-  revert_until RR'.
-  pcofix CIH. i.
-  (* punfold SIM.  *)
-  induction SIM using simg_ind; s.
-  - erewrite ! (bisimulation_is_eq _ _ (map_ret _ _)). eauto with paco.
-  - erewrite ! (bisimulation_is_eq _ _ (map_bind _ _ _)).
-    pfold. apply simg_syscall. i. right. eapply CIH; et.
-    (* specialize (SIM _ _ EQ). pclearbot. et. *)
-    (* edestruct SIM; et. inv H. *)
-  - erewrite ! (bisimulation_is_eq _ _ (map_tau _ _)).
-    pfold. apply simg_tauL; et. punfold IHSIM.
-  - erewrite ! (bisimulation_is_eq _ _ (map_tau _ _)). 
-    pfold. apply simg_tauR; et. punfold IHSIM.
-  - erewrite ! (bisimulation_is_eq _ _ (map_bind _ _ _)).
-    pfold. apply simg_chooseL; et. 
-    des. exists x. punfold IH.
-  - erewrite ! (bisimulation_is_eq _ _ (map_bind _ _ _)).
-    pfold. apply simg_chooseR; et.
-    i. exploit SIM. esplits. des. punfold IH.
-  - erewrite ! (bisimulation_is_eq _ _ (map_bind _ _ _)).
-    pfold. apply simg_takeL; et.
-    i. exploit SIM. esplits. des. punfold IH.
-  - erewrite ! (bisimulation_is_eq _ _ (map_bind _ _ _)).
-    pfold. apply simg_takeR; et.
-    des. exists x. punfold IH.
-  - pfold. apply simg_progress; et. right. eapply CIH; et.
-Qed. *)
